exercises/specifications.v
@@ -1,0 +1,214 @@
+From iris.heap_lang Require Import lang proofmode notation.
+
+(*########## CONTENTS PLAN ##########
+- INTRODUCE WEAKEST-PRECONDITIONS
+  + EXAMPLES WITH BASIC ARITHMETIC
+- INTRODUCE HOARE-TRIPLES
+  + EXAMPLES
+  + RELATIONSHIP TO WP
+  + CONVENTION: HT FOR SPECS, WP FOR PROOFS
+- POSSIBLY MERGE SPECIFICATIONS AND RESOURCES
+  + THEN HAVE EXAMPLES WITH POINTS-TO PREDICATE
+#####################################*)
+
+(** HeapLang is a programming language with an accompanying Iris program
+  logic defined on top of Iris base logic. HeapLang is an untyped
+  higher-order functional programming language with dynamically
+  allocated references and concurrency, in the form of dynamically
+  allocated threads that can share memory access. The evaluation
+  order is right to left and it is a call-by-value language.
+
+  The program logic for HeapLang uses connectives describing locations.
+  These connectives require that certain resources are available. To
+  ensure this, we use the typeclass [heapGS]. This typeclass ensures
+  that Σ contains at least the necessary resources for HeapLang. Later on,
+  we will explain what resources are.
+*)
+Section heaplang.
+Context `{!heapGS Σ}.
+
+(**
+  To see how we can reason about programs written in HeapLang,
+  let us define a small toy program.
+*)
+Definition prog : expr :=
+  (** Allocate the number 1 on the heap *)
+  let: "x" := ref #1 in
+  (** Increment x by 2 *)
+  "x" <- !"x" + #2;;
+  (** Read the value of x *)
+  !"x".
+
+(**
+  This program should evaluate to 3. To prove this we'll use the
+  weakest precondition [WP]. This lets us specify a postcondition we
+  expect to hold if the program halts.
+*)
+Lemma wp_prog : ⊢ WP prog {{ v, ⌜v = #3⌝ }}.
+Proof.
+  rewrite /prog.
+  (**
+    HeapLang has a set of tactics for reasoning about the evaluation of the
+    language. The initial step of prog is to allocate a reference
+    containing the value 1. We can symbolically execute this step of prog by
+    using the [wp_alloc] tactic with a name for the
+    location and a name for the knowledge that the location stores the
+    value 1.
+  *)
+  wp_alloc l as "Hl".
+  (**
+    The next step of prog is a purely functional reduction step, and 
+    and thus we can use [wp_pures] to continue symbolic execution.
+  *)
+  wp_pures.
+  (**
+    Next, we load from the location [l] using the knowledge that it
+    currently stores the value 1.
+  *)
+  wp_load.
+  (** Then we evaluate the addition *)
+  wp_pures.
+  (**
+    Storing is handled by [wp_store].
+    Notice that this updates [Hl]. This only works because we are
+    working in a separation logic.
+  *)
+  wp_store.
+  (** Finally we use [wp_load] again *)
+  wp_load.
+  (**
+    Now that the program has concluded, we are left with a fancy update
+    modality. You can usually ignore this modality and simply introduce
+    it. We will explain its uses as we go along.
+  *)
+  iModIntro.
+  (** Now we are left with a trivial proof that 1 + 2 = 3 *)
+  done.
+Qed.
+
+(**
+  The full list of symbolic evaluation tactics can be found at
+  https://gitlab.mpi-sws.org/iris/iris/-/blob/master/docs/heap_lang.md
+*)
+
+(**
+  Let us use the property we just proved for prog to 
+  prove a specification for a larger program.
+*)
+Lemma wp_prog_add_2 : ⊢ WP prog + #2 {{v, ⌜v = #5⌝}}.
+Proof.
+  iStartProof.
+  (**
+    The first part of this program is to evaluate [prog]. So we can
+    separate the program into 2 parts. First, we evaluate [prog], then
+    we take the result and add 2 to it. To do this we can use [wp_bind].
+  *)
+  wp_bind prog.
+  (**
+    Now we have the problem that our postcondition doesn't match the
+    one we proved. To fix this we can use the monotonicity of WP.
+  *)
+  iApply wp_mono.
+  2: { iApply wp_prog. }
+  iIntros "%_ ->".
+  (** And now we can evaluate the rest of the program *)
+  wp_pures.
+  (** This postcondition is again trivial *)
+  done.
+Qed.
+
+(**
+  The previous proof worked, but it is not very ergonomic.
+  To fix this, we'll make [wp_prog] generic on its postcondition.
+*)
+Lemma wp_prog_2 (Φ : val → iProp Σ) :
+  (∀ v, ⌜v = #3⌝ -∗ Φ v) -∗ WP prog {{v, Φ v}}.
+Proof.
+  iIntros "HΦ".
+  rewrite /prog.
+  wp_alloc l as "Hl".
+  wp_load.
+  wp_store.
+  wp_load.
+  by iApply "HΦ".
+Qed.
+
+(** Now the other proof becomes much simpler. *)
+Lemma wp_prog_add_2_2 : ⊢ WP prog + #2 {{v, ⌜v = #5⌝}}.
+Proof.
+  wp_bind prog.
+  (** Now the proof is on the exact form required by [wp_prog_2] *)
+  iApply wp_prog_2.
+  (** And the proof proceeds as before *)
+  iIntros "%_ ->".
+  by wp_pures.
+Qed.
+
+(**
+  Hoare triples are an extended version of a WP with a 
+  precondition. They are defined as
+  [∀ Φ, Pre -∗ (▷ ∀ r0 .. rn, Post -∗ Φ v) -∗ WP e {{v, Φ v}}].
+  This may seem like a very long and complicated definition, so let's
+  look at it's parts.
+
+  As in the example above, Hoare triples are parameterized on the post conditions
+  satisfied by Post. This allows us to further specialize the
+  possible return values by specifying them as a pattern quantified over
+  arbitrary parameters. The implication of the postcondition is
+  hidden under a later modality (▷), signifying that the program takes at least one
+  step. This modality will be described in the following file.
+  Finally, we have a precondition Pre.
+
+  The syntax for Hoare triples is as follows:
+  [{{{ Pre }}} e {{{ r0 .. rn, RET v; Post }}}]
+  - [Pre]: the precondition that is assumed to hold before the
+    program runs.
+  - [e]: the program to run.
+  - [r0 .. rn]: the parameters used to define the return value.
+  - [v]: an expression specifying the shape of the return value.
+  - [Post]: the postcondition is satisfied after the program has halted.
+*)
+
+(** Let's consider a function that swaps 2 values. *)
+Definition swap : val :=
+  λ: "x" "y",
+  let: "v" := !"x" in
+  "x" <- !"y";;
+  "y" <- "v".
+
+(** To specify this program we can use a Hoare triple. *)
+Lemma wp_swap (l1 l2 : loc) (v1 v2 : val) :
+  {{{l1 ↦ v1 ∗ l2 ↦ v2}}}
+    swap #l1 #l2
+  {{{RET #(); l1 ↦ v2 ∗ l2 ↦ v1}}}.
+Proof.
+  iIntros "%Φ [H1 H2] HΦ".
+  rewrite /swap.
+  wp_pures.
+  wp_load.
+  wp_load.
+  wp_store.
+  wp_store.
+  iApply "HΦ".
+  by iFrame.
+Qed.
+
+(**
+  And we can use this specification to prove the correctness of the
+  client code.
+*)
+Lemma swap_swap (l1 l2 : loc) (v1 v2 : val) :
+  {{{l1 ↦ v1 ∗ l2 ↦ v2}}}
+    swap #l1 #l2;; swap #l1 #l2
+  {{{RET #(); l1 ↦ v1 ∗ l2 ↦ v2}}}.
+Proof.
+  iIntros "%Φ [H1 H2] HΦ".
+  wp_bind (swap _ _).
+  iApply (wp_swap with "[$H1 $H2]").
+  iIntros "!> [H1 H2]".
+  wp_pures.
+  iApply (wp_swap with "[$H1 $H2]").
+  done.
+Qed.
+
+End heaplang.
